Clean up focus tactics

mechanization/tactics/Focus.v
@@ -1,5 +1,18 @@
 From Warblre Require Import Result.
 
+(** Focus allows to act on a specific sub term of an hypothesis or goal.
+
+    The idea behind this family of tactics is to allow the user to specify
+    a part of an hypothesis or goal to which apply a tactic, as opposed to applying it to the whole hypothesis/goal.
+
+    E.g.
+    Assuming an hypothesis
+    H: R (a + b) c
+    on can use
+    focus <! _ [] _ !> print in H.
+    to print (a + b).
+*)
+
 Inductive focus :=
 | Here
 | AppL (f: focus)
@@ -7,205 +20,11 @@ Inductive focus :=
 | ArrowL (f: focus)
 | ArrowR (f: focus)
 | IteCond (f: focus)
-| LetBound (f: focus)
-| FunR (f: focus).
+| LetBound (f: focus).
 
-Fixpoint focus_insert (f inserted: focus) := match f with
-| Here => inserted
-| AppL f' => AppL (focus_insert f' inserted)
-| AppR f' => AppR (focus_insert f' inserted)
-| ArrowL f' => ArrowL (focus_insert f' inserted)
-| ArrowR f' => ArrowR (focus_insert f' inserted)
-| IteCond f' => IteCond (focus_insert f' inserted)
-| LetBound f' => LetBound (focus_insert f' inserted)
-| FunR f' => FunR (focus_insert f' inserted)
-end.
-
-
-(* Ltac red_tl_beta t := (eval simpl ((fun _ => _) _) at 1 in t).
-Ltac red_tl_ite t := (eval simpl (if _ then _ else _) at 1 in t). *)
-
-
-
-Ltac assert_type t T := lazymatch type of t with
-| T => idtac
-| ?T' => fail 99 "Epected type" T "got" T'
-end.
-
-Ltac focus_excise f t :=
-  let _ := assert_type f focus in
-  let rec iter f t := lazymatch f with
-  | Here => lazymatch t with ?g => g end
-  | AppL ?f' => lazymatch t with ?t' _ => iter f' t' end
-  | AppR ?f' => lazymatch t with _ ?t' => iter f' t' end
-  | ArrowL ?f' => lazymatch t with ?t' -> _ => iter f' t' end
-  | ArrowR ?f' => lazymatch t with _ -> ?t' => iter f' t' end
-  | IteCond ?f' => lazymatch t with if ?t' then _ else _ => iter f' t' end
-  | LetBound ?f' => lazymatch t with let _ := ?t' in _ => iter f' t' end
-  | FunR ?f' => lazymatch t with fun x => ?t' => iter f' t' end
-  | _ => fail 100 "Unknown focus" f
-  end in
-  iter f t.
-
-Ltac focus_replace f t r :=
-  let _ := assert_type f focus in
-  let rec iter f t r := lazymatch f with
-  | Here => let t' := r t in t'
-  | AppL ?f' => lazymatch t with ?t' ?o => let t'' := iter f' t' r in constr:(t'' o) end
-  | AppR ?f' => lazymatch t with ?o ?t' => let t'' := iter f' t' r in constr:(o t'') end
-  | ArrowL ?f' => lazymatch t with ?t' -> ?o => let t'' := iter f' t' r in constr:(t'' -> o) end
-  | ArrowR ?f' => lazymatch t with ?o -> ?t' => let t'' := iter f' t' r in constr:(o -> t'') end
-  | IteCond ?f' => lazymatch t with if ?t' then ?thenn else ?elze => let t'' := iter f' t' r in constr:(if t'' then thenn else elze) end
-  | LetBound ?f' => lazymatch t with let x := ?t' in ?o => 
-    let t'' := iter f' t' r in
-    let s := constr:(let x := t'' in o) in
-    s
-    end
-  | FunR ?f' => lazymatch t with fun x => ?t' => 
-    let t'' := iter f' t' r in
-    let s := constr:(fun x => t'') in
-    s
-    end
-  | _ => fail 100 "Unknown focus" f
-  end in
-  iter f t r.
-
-Ltac focus_get_goal := lazymatch goal with [ |- ?g ] => g end.
-Ltac focus_get_hypothesis H := match type of H with ?T => T end.
-Ltac focus_get_focus := match goal with
-| [ _ := [?f] : focus |- _ ] => f
-end.
-Ltac focus_clear_focus := match goal with
-| [ focus := [?f] : focus |- _ ] => clear focus
-| [ |- _ ] => idtac
-end.
-
-(*  Replace has the bad habit of applying some transformation (cbn? hnf?)
-    to the replacement, so we apply the same transformation to the goal to ensure
-    perfect matching. *)
-Ltac focus_replace_goal With By :=
-  cbn;
-  let g := focus_get_goal in
-  replace g with With;
-  [ idtac | By ].
-Ltac focus_replace_hypothesis H With By :=
-  cbn in H;
-  let g := focus_get_hypothesis H in
-  replace g with With in H;
-  [ idtac | By ].
-
-Ltac destruct_or_rewrite t := lazymatch goal with
-| [ H: t = ?v |- _ ] => rewrite -> H
-| [ |- _ ] => let Eq := fresh "AutoDest_" in destruct t eqn:Eq
-end.
-
-Ltac auto_destruct t := lazymatch t with
-| Result.bind ?c _ => 
-    destruct_or_rewrite c;
-    match goal with
-    | [ _: c = ?v |- _ ] => simpl (Result.bind v _) in *
-    end
-| match ?c with | _ => _ end => destruct_or_rewrite c
-| if ?c then _ else _ => destruct_or_rewrite c
-| ?l _ => auto_destruct l
-end; try discriminate.
-
-Tactic Notation "focus" constr(f) "do" tactic(t) := (
-  assert_type f focus;
-  let g := focus_get_goal in
-  let focused := focus_excise f g in
-  t focused).
-Tactic Notation "focus" constr(f) "print" := (
-  let t := (fun t => idtac t) in
-  focus f do t).
-Tactic Notation "focus" constr(f) "replace" "using" tactic(t) "by" tactic(s) := (
-  assert_type f focus;
-  let g := focus_get_goal in
-  let replacement := focus_replace f g t in
-  focus_replace_goal replacement ltac:(solve [ s ])).
-Tactic Notation "focus" constr(f) "replace" "using" tactic(t) := (
-  assert_type f focus;
-  let g := focus_get_goal in
-  let replacement := focus_replace f g t in
-  focus_replace_goal replacement ltac:(try reflexivity)).
-Tactic Notation "focus" constr(f) "replace" "with" constr(r) := (
-  let r' := (fun _ => r) in
-  focus f replace using r').
-Tactic Notation "focus" constr(f) "replace" "with" constr(r) "by" tactic(s) := (
-  let r' := (fun _ => r) in
-  focus f replace using r' by s).
-Tactic Notation "focus" constr(f) "auto" "destruct" := (
-  assert_type f focus;
-  repeat(
-    let g := focus_get_goal in
-    let t := focus_excise f g in
-    auto_destruct t)).
-
-Tactic Notation "focus" constr(f) "do" tactic(t) "in" hyp(H) := (
-  assert_type f focus;
-  let g := focus_get_hypothesis H in
-  let focused := focus_excise f g in
-  t focused).
-Tactic Notation "focus" constr(f) "print" "in" hyp(H) := (
-  let t := (fun t => idtac t) in
-  focus f do t in H).
-Tactic Notation "focus" constr(f) "replace" "using" tactic(t) "by" tactic(s) "in" hyp(H) := (
-  assert_type f focus;
-  let g := focus_get_hypothesis H in
-  let replacement := focus_replace f g t in
-  focus_replace_hypothesis H replacement ltac:(solve [ s ])).
-Tactic Notation "focus" constr(f) "replace" "using" tactic(t) "in" hyp(H) := (
-  assert_type f focus;
-  let g := focus_get_hypothesis H in
-  let replacement := focus_replace f g t in
-  focus_replace_hypothesis H replacement ltac:(try reflexivity)).
-Tactic Notation "focus" constr(f) "replace" "with" constr(r) "in" hyp(H) := (
-  let r' := (fun _ => r) in
-  focus f replace using r' in H).
-Tactic Notation "focus" constr(f) "remember" "as" simple_intropattern(I) "in" hyp(H) := (
-  let r := (fun t => remember t as I) in
-  focus f do r in H).
-Tactic Notation "focus" constr(f) "replace" "with" constr(r) "by" tactic(s) "in" hyp(H) := (
-  let r' := (fun _ => r) in
-  focus f replace using r' by s in H).
-Tactic Notation "focus" constr(f) "auto" "destruct" "in" hyp(H) := (
-  assert_type f focus;
-  repeat(
-    let g := focus_get_hypothesis H in
-    let t := focus_excise f g in
-    auto_destruct t)).
-
-Tactic Notation "focused" "set" constr(f) := (
-  assert_type f focus;
-  focus_clear_focus;
-  set (focus := f)).
-
-
-Tactic Notation "focused" "do" tactic(t) := (
-  let f := focus_get_focus in
-  focus f do t).
-Tactic Notation "focused" "print" := (
-  let f := focus_get_focus in
-  focus f print).
-Tactic Notation "focused" "replace" "using" tactic(t) "by" tactic(s) := (
-  let f := focus_get_focus in
-  focus f replace using t by s).
-Tactic Notation "focused" "replace" "using" tactic(t) := (
-  let f := focus_get_focus in
-  focus f replace using t).
-Tactic Notation "focused" "replace" "with" constr(r) := (
-  let f := focus_get_focus in
-  focus f replace with r).
-Tactic Notation "focus" constr(f) "remember" "as" simple_intropattern(I) := (
-  let r := (fun t => remember t as I) in
-  focus f do r).
-Tactic Notation "focused" "replace" "with" constr(r) "by" tactic(s) := (
-  let f := focus_get_focus in
-  focus f replace with r by s).
-
-
+(** Grammar to write focuses. *)
 Declare Custom Entry focus.
-Notation "'§' e '§'" := e (e custom focus at level 99).
+Notation "'<!' e '!>'" := e (e custom focus at level 99).
 Notation "'[]'" := Here (in custom focus at level 0).
 Notation "'(' f ')'" := f (in custom focus at level 0, f at level 99).
 Notation "'if' f 'then' '_' 'else' '_'" := (IteCond f) (in custom focus at level 99).
@@ -223,9 +42,136 @@ Notation "'_' '_' '_' '_' '_' '_' '_' f" := (AppR f) (in custom focus at level 5
 Notation "'_' '_' '_' '_' '_' '_' '_' '_' f" := (AppR f) (in custom focus at level 50, f at level 49, left associativity, only parsing).
 Notation "'_' '_' '_' '_' '_' '_' '_' '_' '_' f" := (AppR f) (in custom focus at level 50, f at level 49, left associativity, only parsing).
 Notation "'_' '_' '_' '_' '_' '_' '_' '_' '_' '_' f" := (AppR f) (in custom focus at level 50, f at level 49, left associativity, only parsing).
-Notation "'fun' '_' '=>' f" := (FunR f) (in custom focus at level 99, right associativity).
-Notation "'fun' '_' '_' '=>' f" := (FunR (FunR f)) (in custom focus at level 99, right associativity).
-Notation "'fun' '_' '_' '_' '=>' f" := (FunR (FunR (FunR f))) (in custom focus at level 99, right associativity).
-Notation "'fun' '_' '_' '_' '_' '=>' f" := (FunR (FunR (FunR (FunR f)))) (in custom focus at level 99, right associativity).
-Notation "'fun' '_' '_' '_' '_' '_' '=>' f" := (FunR (FunR (FunR (FunR (FunR f))))) (in custom focus at level 99, right associativity).
-Notation "'fun' '_' '_' '_' '_' '_' '_' '=>' f" := (FunR (FunR (FunR (FunR (FunR (FunR f)))))) (in custom focus at level 99, right associativity).
+
+(** Internal implementation *)
+Local Fixpoint focus_insert (f inserted: focus) := match f with
+| Here => inserted
+| AppL f' => AppL (focus_insert f' inserted)
+| AppR f' => AppR (focus_insert f' inserted)
+| ArrowL f' => ArrowL (focus_insert f' inserted)
+| ArrowR f' => ArrowR (focus_insert f' inserted)
+| IteCond f' => IteCond (focus_insert f' inserted)
+| LetBound f' => LetBound (focus_insert f' inserted)
+end.
+
+Local Ltac assert_type t T := lazymatch type of t with
+| T => idtac
+| ?T' => fail 99 "Epected type" T "got" T'
+end.
+
+Local Ltac focus_excise f t :=
+  let _ := assert_type f focus in
+  let rec iter f t := lazymatch f with
+  | Here => lazymatch t with ?g => g end
+  | AppL ?f' => lazymatch t with ?t' _ => iter f' t' end
+  | AppR ?f' => lazymatch t with _ ?t' => iter f' t' end
+  | ArrowL ?f' => lazymatch t with ?t' -> _ => iter f' t' end
+  | ArrowR ?f' => lazymatch t with _ -> ?t' => iter f' t' end
+  | IteCond ?f' => lazymatch t with if ?t' then _ else _ => iter f' t' end
+  | LetBound ?f' => lazymatch t with let _ := ?t' in _ => iter f' t' end
+  | _ => fail 100 "Unknown focus" f
+  end in
+  iter f t.
+
+Local Ltac focus_replace f t r :=
+  let _ := assert_type f focus in
+  let rec iter f t r := lazymatch f with
+  | Here => let t' := r t in t'
+  | AppL ?f' => lazymatch t with ?t' ?o => let t'' := iter f' t' r in constr:(t'' o) end
+  | AppR ?f' => lazymatch t with ?o ?t' => let t'' := iter f' t' r in constr:(o t'') end
+  | ArrowL ?f' => lazymatch t with ?t' -> ?o => let t'' := iter f' t' r in constr:(t'' -> o) end
+  | ArrowR ?f' => lazymatch t with ?o -> ?t' => let t'' := iter f' t' r in constr:(o -> t'') end
+  | IteCond ?f' => lazymatch t with if ?t' then ?thenn else ?elze => let t'' := iter f' t' r in constr:(if t'' then thenn else elze) end
+  | LetBound ?f' => lazymatch t with let x := ?t' in ?o => 
+    let t'' := iter f' t' r in
+    let s := constr:(let x := t'' in o) in
+    s
+    end
+  | _ => fail 100 "Unknown focus" f
+  end in
+  iter f t r.
+
+Local Ltac focus_get_goal := lazymatch goal with [ |- ?g ] => g end.
+Local Ltac focus_get_hypothesis H := match type of H with ?T => T end.
+Local Ltac focus_get_focus := match goal with
+| [ _ := [?f] : focus |- _ ] => f
+end.
+Local Ltac focus_clear_focus := match goal with
+| [ focus := [?f] : focus |- _ ] => clear focus
+| [ |- _ ] => idtac
+end.
+
+(*  Replace has the bad habit of applying some transformation (cbn? hnf?)
+    to the replacement, so we apply the same transformation to the goal to ensure
+    perfect matching. *)
+Local Ltac focus_replace_goal With By :=
+  cbn;
+  let g := focus_get_goal in
+  replace g with With;
+  [ idtac | By ].
+Local Ltac focus_replace_hypothesis H With By :=
+  cbn in H;
+  let g := focus_get_hypothesis H in
+  replace g with With in H;
+  [ idtac | By ].
+
+Local Ltac destruct_or_rewrite t := lazymatch goal with
+| [ H: t = ?v |- _ ] => rewrite -> H
+| [ |- _ ] => let Eq := fresh "AutoDest_" in destruct t eqn:Eq
+end.
+
+Local Ltac auto_destruct t := lazymatch t with
+| Result.bind ?c _ => 
+    destruct_or_rewrite c;
+    match goal with
+    | [ _: c = ?v |- _ ] => simpl (Result.bind v _) in *
+    end
+| match ?c with | _ => _ end => destruct_or_rewrite c
+| if ?c then _ else _ => destruct_or_rewrite c
+| ?l _ => auto_destruct l
+end; try discriminate.
+
+(** User-facing tactics *)
+
+(* Call t with the focused term. *)
+Tactic Notation "focus" constr(f) "do" tactic(t) := (
+  assert_type f focus;
+  let g := focus_get_goal in
+  let focused := focus_excise f g in
+  t focused).
+(* Print the focused term *)
+Tactic Notation "focus" constr(f) "print" := (
+  let t := (fun t => idtac t) in
+  focus f do t).
+(* Replace the focused term by a variable, and introduce an hypothesis about that variable's definition. *)
+Tactic Notation "focus" constr(f) "remember" "as" simple_intropattern(I) "with" "equality" simple_intropattern(J) := (
+  let r := (fun t => remember t as I eqn:J) in
+  focus f do r).
+(* Auto destructs the focused term.
+   This means that if the 'head' of the focused term is of the form
+    - match t with ... => t is destructed
+    - if t then ... => t is destructed
+    - let! _ =<< t in ... => t is destructed
+*)
+Tactic Notation "focus" constr(f) "auto" "destruct" := (
+  assert_type f focus;
+  repeat(
+    let g := focus_get_goal in
+    let t := focus_excise f g in
+    auto_destruct t)).
+
+(* These tactics are the same, but target an hypothesis instead *)
+Tactic Notation "focus" constr(f) "do" tactic(t) "in" hyp(H) := (
+  assert_type f focus;
+  let g := focus_get_hypothesis H in
+  let focused := focus_excise f g in
+  t focused).
+Tactic Notation "focus" constr(f) "print" "in" hyp(H) := (
+  let t := (fun t => idtac t) in
+  focus f do t in H).
+Tactic Notation "focus" constr(f) "auto" "destruct" "in" hyp(H) := (
+  assert_type f focus;
+  repeat(
+    let g := focus_get_hypothesis H in
+    let t := focus_excise f g in
+    auto_destruct t)).
