mechanization/tactics/Retrieve.v
@@ -1,12 +1,14 @@
 Require Import Ltac2.Ltac2.
 From Ltac2 Require Import Control Pattern List.
 
-(** TODO: once updated to a newer version (1.19.0?) supporting https://github.com/coq/coq/pull/18690,
-          remove and use builtin.
+(*  TODO:
+    once updated to a newer version (8.20?) supporting https://github.com/coq/coq/pull/18690,
+    remove and use builtin.
 *)
 Ltac2 numgoals (_: unit): int :=
   1.
 
+(** A tactic to retrieve an hypothesis by the shape of its type. *)
 Ltac2 retrieve (pat: pattern) (into: ident): unit :=
   let hyp_patterns := (None, (Pattern.MatchPattern, pat)) :: [] in
   let goal_pattern := (Pattern.MatchPattern, pat:(_)) in
